Reorganize modules + executable memory model module.

src/coq/Handlers/MemoryModel.v
@@ -8,6 +8,9 @@ From Vellvm.Semantics Require Import
      LLVMParams
      LLVMEvents.
 
+From Vellvm.Handlers Require Import
+     MemPropT.
+
 From Vellvm.Utils Require Import
      Error
      PropT.
@@ -25,49 +28,40 @@ From ITree Require Import
      Events.State.
 
 From Coq Require Import
-     ZArith.
+     ZArith
+     Strings.String
+     List.
+
+Import ListNotations.
+Import ListUtil.
+Import Utils.Monads.
 
 Import Basics.Basics.Monads.
 Import MonadNotation.
 Open Scope monad_scope.
 
-(* Move this ? *)
-Definition store_id := N.
-Class MonadStoreID (M : Type -> Type) : Type :=
-  { fresh_sid : M store_id;
-  }.
 
-Class MonadMemState (MemState : Type) (M : Type -> Type) : Type :=
-  { get_mem_state : M MemState;
-    put_mem_state : MemState -> M unit;
-  }.
-
-Definition modify_mem_state {M MemState} `{Monad M} `{MonadMemState MemState M} (f : MemState -> MemState) : M MemState :=
-  ms <- get_mem_state;;
-  put_mem_state (f ms);;
-  ret ms.
-
-(* TODO: Add RAISE_PICK or something... May need to be in a module *)
-Class MemMonad (MemState : Type) (AllocationId : Type) (M : Type -> Type)
-      `{Monad M}
-      `{MonadAllocationId AllocationId M} `{MonadStoreID M} `{MonadMemState MemState M}
-      `{RAISE_ERROR M} `{RAISE_UB M} `{RAISE_OOM M} : Type
-  :=
-  {
-    MemMonad_runs_to_prop {A} (ma : M A) (ms : MemState) (res : OOM (MemState * A)) : Prop;
-    MemMonad_runs_to {A} (ma : M A) (ms : MemState) : option (MemState * A);
-    MemMonad_lift_stateT
-      {E} `{FailureE -< E} `{UBE -< E} `{OOME -< E} {A}
-      (ma : M A) : stateT MemState (itree E) A;
-  }.
-
-(* Module types for memory models to allow different memory models to be plugged in. *)
-Module Type MemoryModel (LP : LLVMParams) (MP : MemoryParams LP).
+Module Type MemoryModelSpecPrimitives (LP : LLVMParams) (MP : MemoryParams LP).
   Import LP.Events.
   Import LP.ADDR.
   Import LP.SIZEOF.
-
   Import LP.PROV.
+
+  Require Import MemBytes.
+  Module MemByte := Byte LP.ADDR LP.IP LP.SIZEOF LP.Events MP.BYTE_IMPL.
+  Import MemByte.
+  Import LP.SIZEOF.
+
+  (*** Internal state of memory *)
+  Parameter MemState : Type.
+  Parameter initial_memory_state : MemState.
+
+  (* Type for frames and frame stacks *)
+  Parameter Frame : Type.
+  Parameter FrameStack : Type.
+
+  Parameter initial_frame : Frame.
+
   (* TODO: Should DataLayout be here?
 
      It might make sense to move DataLayout to another module, some of
@@ -79,298 +73,94 @@ Module Type MemoryModel (LP : LLVMParams) (MP : MemoryParams LP).
    *)
   (* Parameter datalayout : DataLayout. *)
 
-  (** Datatype for the state of memory *)
-  Parameter MemState : Type.
-  Parameter initial_memory_state : MemState.
+  (*** Primitives on memory *)
 
-  Definition MemStateT := stateT MemState.
+  (** Reads *)
+  Parameter read_byte_MemPropT : addr -> MemPropT MemState SByte.
 
-  Instance MemStateT_MonadAllocationId {M} :
-    MonadAllocationId AllocationId (MemStateT M).
-  Proof.
-  Admitted.
+  (** Allocations *)
+  (* Returns true if a byte is allocated with a given AllocationId? *)
+  Parameter addr_allocated_prop : addr -> AllocationId -> MemPropT MemState bool.
 
-  Instance MemStateT_MonadStoreID {M} :
-    MonadStoreID (MemStateT M).
-  Proof.
-  Admitted.
+  (** Frame stacks *)
+  (* Check if an address is allocated in a frame *)
+  Parameter ptr_in_frame_prop : Frame -> addr -> Prop.
 
-  Instance MemStateT_MonadMemState {M} :
-    MonadMemState MemState (MemStateT M).
-  Proof.
-    split.
-    eapply (MonadState.get).
-    eapply (MonadState.put).
-  Admitted.
+  (* Check for the current frame *)
+  Parameter peek_frame_stack_prop : FrameStack -> Frame -> Prop.
+  Parameter pop_frame_stack_prop : FrameStack -> FrameStack -> Prop.
 
-  Parameter free_concrete_space :
-    forall (ms : MemState) (phys_addr : Z) (sz : N), bool.
+  Parameter mem_state_frame_stack_prop : MemState -> FrameStack -> Prop.
 
-  Definition concrete_memory_pick_post
-             (st : MemState * (addr * dtyp)) (phys_addr : Z) : Prop
-    := match st with
-       | (ms, (a, dt)) =>
-           free_concrete_space ms phys_addr (sizeof_dtyp dt) = true
-       end.
+  (** Allocation ids / store ids *)
+  Parameter used_allocation_id_prop : MemState -> AllocationId -> Prop.
+  Parameter used_store_id_prop : MemState -> store_id -> Prop.
+End MemoryModelSpecPrimitives.
 
-  Definition PickConcreteMemoryE :=
-    @PickE (MemState * (addr * dtyp)) Z concrete_memory_pick_post.
+Module MemoryHelpers (LP : LLVMParams) (MP : MemoryParams LP).
+  (*** Other helpers *)
+  Import MP.GEP.
+  Import MP.BYTE_IMPL.
+  Import LP.
+  Import LP.ADDR.
+  Import LP.Events.
+  Import LP.SIZEOF.
 
-  (* Not sure if we need this yet *)
-  Parameter free_logical_space :
-    forall (ms : MemState) (ptr : addr) (sz : N), bool.
+  (* TODO: Move this? *)
+  Definition intptr_seq (start : Z) (len : nat) : OOM (list IP.intptr)
+    := Util.map_monad (IP.from_Z) (Zseq start len).
 
-  Definition PickLogicalMemoryE :=
-    @PickE (MemState * dtyp) addr
-           (fun '(ms, dt) ptr =>
-              free_logical_space ms ptr (sizeof_dtyp dt) = true).
+  Definition get_consecutive_ptrs {M} `{Monad M} `{RAISE_OOM M} `{RAISE_ERROR M} (ptr : addr) (len : nat) : M (list addr) :=
+    ixs <- lift_OOM (intptr_seq 0 len);;
+    lift_err_RAISE_ERROR
+      (Util.map_monad
+         (fun ix => handle_gep_addr (DTYPE_I 8) ptr [DVALUE_IPTR ix])
+         ixs).
 
-  Instance MemStateT_itree_MemMonad
-           {E} `{FailureE -< E} `{UBE -< E} `{OOME -< E} `{PickConcreteMemoryE -< E}
-    : MemMonad MemState AllocationId (MemStateT (itree E)).
-  Admitted.
+  Definition generate_undef_bytes (dt : dtyp) (sid : store_id) : OOM (list SByte) :=
+    N.recursion
+      (fun (x : N) => ret [])
+      (fun n mf x =>
+         rest_bytes <- mf (N.succ x);;
+         x' <- IP.from_Z (Z.of_N x);;
+         let byte := uvalue_sbyte (UVALUE_Undef dt) dt (UVALUE_IPTR x') sid in
+         ret (byte :: rest_bytes))
+      (sizeof_dtyp dt) 0%N.
+End MemoryHelpers.
 
-  (* (** MemMonad *) *)
-  (* Parameter MemMonad : Type -> Type. *)
-
-  (* (** Extra monad classes *) *)
-  (* Parameter MemMonad_MonadStoreID : MonadStoreID MemMonad. *)
-  (* Parameter MemMonad_MonadProvenance : MonadProvenance Provenance MemMonad. *)
-  (* Parameter MemMonad_MonadMemState : MonadMemState MemState MemMonad. *)
-
-  (* Parameter MemMonad_RAISE_ERROR : RAISE_ERROR MemMonad. *)
-  (* Parameter MemMonad_RAISE_UB : RAISE_UB MemMonad. *)
-  (* Parameter MemMonad_RAISE_OOM : RAISE_OOM MemMonad. *)
-  (* Parameter MemMonad_RAISE_PICK : RAISE_PICK MemMonad. *)
-
-  (* (* Hack to make typeclass resolution work... *) *)
-  (* Hint Resolve MemMonad_MonadStoreID : typeclass_instances. *)
-  (* Hint Resolve MemMonad_MonadProvenance : typeclass_instances. *)
-  (* Hint Resolve MemMonad_MonadMemState : typeclass_instances. *)
-  (* Hint Resolve MemMonad_RAISE_ERROR : typeclass_instances. *)
-  (* Hint Resolve MemMonad_RAISE_UB : typeclass_instances. *)
-  (* Hint Resolve MemMonad_RAISE_OOM : typeclass_instances. *)
-  (* Hint Resolve MemMonad_RAISE_PICK : typeclass_instances. *)
-
-  (* Parameter MemMonad_runs_to : forall {A} (ma : MemMonad A) (ms : MemState), option (MemState * A). *)
-  (* Parameter MemMonad_lift_stateT :  *)
-  (*   forall {E} `{FailureE -< E} `{UBE -< E} `{OOME -< E} `{PickE -< E} {A} *)
-  (*     (ma : MemMonad A), stateT MemState (itree E) A. *)
-
-  (** Basic operations on the state of logical memory. *)
-  Parameter allocate :
-    forall {M} `{MemMonad MemState Provenance M} (dt : dtyp),
-      M addr.
-
-  Parameter allocated :
-    forall {M} `{MemMonad MemState Provenance M} (ptr : addr),
-      M bool.
-
-  Parameter read :
-    forall {M} `{MemMonad MemState Provenance M} (ptr : addr) (t : dtyp), M uvalue.
-
-  Parameter write :
-    forall {M} `{MemMonad MemState Provenance M}
-      (ptr : addr) (v : uvalue) (t : dtyp),
-      M unit.
-
-  (** Operations for interacting with the concrete layout of memory. *)
-  Parameter reserve_block : MemState -> LP.IP.intptr -> N -> option MemState.
-
-  Section Handlers.
-    (* TODO: Should we generalize the return type? *)
-    Parameter handle_memory :
-      forall {M} `{MemMonad MemState Provenance M},
-      MemoryE ~> M.
-
-    Parameter handle_intrinsic :
-      forall {M} `{MemMonad MemState Provenance M},
-      IntrinsicE ~> M.
-   End Handlers.
-End MemoryModel.
-
-Module MemoryState (LP : LLVMParams) (MP : MemoryParams LP).
-
-End MemoryState.
-
-Module MemoryModelSpec (LP : LLVMParams) (MP : MemoryParams LP).
+Module Type MemoryModelSpec (LP : LLVMParams) (MP : MemoryParams LP) (MMSP : MemoryModelSpecPrimitives LP MP).
+  Import LP.
   Import LP.Events.
   Import LP.ADDR.
   Import LP.SIZEOF.
   Import LP.PROV.
+  Import MMSP.
 
   Require Import MemBytes.
+
   Module MemByte := Byte LP.ADDR LP.IP LP.SIZEOF LP.Events MP.BYTE_IMPL.
   Import MemByte.
-  Import LP.SIZEOF.
 
-  Parameter MemState : Type.
-  Definition MemPropT (X: Type): Type :=
-    MemState -> err (OOM (MemState * X)%type) -> Prop.
+  Module MemHelpers := MemoryHelpers LP MP.
+  Import MemHelpers.
 
-  (* Instance MemPropT_Monad : Monad MemPropT. *)
-  (* Proof. *)
-  (*   split. *)
-  (*   - (* ret *) *)
-  (*     intros T x. *)
-  (*     unfold MemPropT. *)
-  (*     intros ms [err_msg | [[ms' res] | oom_msg]]. *)
-  (*     + exact False. (* error is not a valid behavior here *) *)
-  (*     + exact (ms = ms' /\ x = res). *)
-  (*     + exact True. (* Allow OOM to refine anything *) *)
-  (*   - (* bind *) *)
-  (*     intros A B ma amb. *)
-  (*     unfold MemPropT in *. *)
+  Definition read_byte_prop (ms : MemState) (ptr : addr) (byte : SByte) : Prop
+    := read_byte_MemPropT ptr ms (inr (NoOom (ms, byte))).
 
-  (*     intros ms [err_msg | [[ms'' b] | oom_msg]]. *)
-  (*     + (* an error is valid when ma errors, or the continuation errors... *) *)
-  (*       refine *)
-  (*         ((exists err, ma ms (inl err)) \/ *)
-  (*          (exists ms' a, *)
-  (*              ma ms (inr (NoOom (ms', a))) -> *)
-  (*              (exists err, amb a ms' (inl err)))). *)
-  (*     + (* No errors, no OOM *) *)
-  (*       refine *)
-  (*         (exists ms' a k, *)
-  (*             ma ms (inr (NoOom (ms', a))) -> *)
-  (*             amb a ms' (inr (NoOom (ms'', k a)))). *)
-  (*     + (* OOM is always valid *) *)
-  (*       exact True. *)
-  (* Defined. *)
+  Definition byte_allocated_MemPropT (ptr : addr) (aid : AllocationId) : MemPropT MemState unit :=
+    m <- get_mem_state;;
+    b <- addr_allocated_prop ptr aid;;
+    MemPropT_assert (b = true).
 
-  (* To triple check, but the following makes more sense to me *)
-  Instance MemPropT_Monad : Monad MemPropT.
-  Proof.
-    split.
-    - (* ret *)
-      refine (fun _ v s r => match r with
-                          | inl _ => False
-                          | inr (NoOom (s',r')) => s' = s /\ r' = v
-                          | inr (Oom _) => True
-                          end).
-    - (* bind *)
-      refine (fun A B ma amb sa r =>
-                match r with
-                | inl err            =>
-                    ma sa (inl err) \/
-                      (exists sab a, ma sa (inr (NoOom (sab, a))) /\
-                                  (exists err, amb a sab (inl err)))
-                | inr (NoOom (sb,r)) =>
-                    exists sab a,
-                    ma    sa  (inr (NoOom (sab, a))) /\
-                      amb a sab (inr (NoOom (sb, r)))
-                | inr (Oom _)         => True
-                end
-             ).
-  Defined.
+  Definition byte_allocated (ms : MemState) (ptr : addr) (aid : AllocationId) : Prop
+    := byte_allocated_MemPropT ptr aid ms (inr (NoOom (ms, tt))).
 
-  Instance MemPropT_MonadMemState : MonadMemState MemState MemPropT.
-  Proof.
-    split.
-    - (* get_mem_state *)
-      unfold MemPropT.
-      intros ms [err_msg | [[ms' a] | oom_msg]].
-      + exact True.
-      + exact (ms = ms' /\ a = ms).
-      + exact True.
-    - (* put_mem_state *)
-      unfold MemPropT.
-      intros ms_to_put ms [err_msg | [[ms' t] | oom_msg]].
-      + exact True.
-      + exact (ms_to_put = ms').
-      + exact True.
-  Defined.
-
-  Instance MemPropT_RAISE_OOM : RAISE_OOM MemPropT.
-  Proof.
-    split.
-    - intros A msg.
-      unfold MemPropT.
-      intros ms [err | [_ | oom]].
-      + exact False. (* Must run out of memory, can't error *)
-      + exact False. (* Must run out of memory *)
-      + exact True. (* Don't care about message *)
-  Defined.
-
-  Instance MemPropT_RAISE_ERROR : RAISE_ERROR MemPropT.
-  Proof.
-    split.
-    - intros A msg.
-      unfold MemPropT.
-      intros ms [err | [_ | oom]].
-      + exact True. (* Any error will do *)
-      + exact False. (* Must error *)
-      + exact False. (* Must error *)
-  Defined.
-
-  Definition MemPropT_assert {X} (assertion : Prop) : MemPropT X
-    := fun ms ms'x =>
-         match ms'x with
-         | inl _ =>
-             assertion
-         | inr (NoOom (ms', x)) =>
-             ms = ms' /\ assertion
-         | inr (Oom s) =>
-             assertion
-         end.
-
-  Definition MemPropT_assert_post {X} (Post : X -> Prop) : MemPropT X
-    := fun ms ms'x =>
-         match ms'x with
-         | inl _ =>
-             True
-         | inr (NoOom (ms', x)) =>
-             ms = ms' /\ Post x
-         | inr (Oom s) =>
-             True
-         end.
-
-  Section Handlers.
-    Variable (E F: Type -> Type).
-    Context `{FailureE -< E}.
-
-    Variable MemM : Type -> Type.
-    Context `{MemM_MemMonad : MemMonad MemState Provenance MemM}.
+  Definition byte_not_allocated (ms : MemState) (ptr : addr) : Prop
+    := forall (aid : AllocationId), ~ byte_allocated ms ptr aid.
 
     (** Addresses *)
     Definition disjoint_ptr_byte (a b : addr) :=
       ~ ptr_overlap a b.
-
-    (*** Primitives *)
-
-    (** Reads *)
-    Parameter read_byte_MemPropT : addr -> MemPropT SByte.
-    Definition read_byte_prop (ms : MemState) (ptr : addr) (byte : SByte) : Prop
-      := read_byte_MemPropT ptr ms (inr (NoOom (ms, byte))).
-
-    (** Allocations *)
-    (* Is a byte allocated with a given AllocationId? *)
-    Parameter addr_allocated_prop : addr -> AllocationId -> MemPropT bool.
-
-    Definition byte_allocated_MemPropT (ptr : addr) (aid : AllocationId) : MemPropT unit :=
-      m <- get_mem_state;;
-      b <- addr_allocated_prop ptr aid;;
-      MemPropT_assert (b = true).
-
-    Definition byte_allocated (ms : MemState) (ptr : addr) (aid : AllocationId) : Prop
-      := byte_allocated_MemPropT ptr aid ms (inr (NoOom (ms, tt))).
-
-    Definition byte_not_allocated (ms : MemState) (ptr : addr) : Prop
-      := forall (aid : AllocationId), ~ byte_allocated ms ptr aid.
-
-    (** Frame stacks *)
-    Parameter Frame : Type.
-    Parameter ptr_in_frame : Frame -> addr -> Prop.
-
-    Parameter FrameStack : Type.
-    Parameter peek_frame_stack : FrameStack -> Frame -> Prop.
-    Parameter pop_frame_stack : FrameStack -> FrameStack -> Prop.
-
-    Parameter mem_state_frame_stack : MemState -> FrameStack -> Prop.
-
-    (** Allocation ids / store ids *)
-    Parameter used_allocation_id : MemState -> AllocationId -> Prop.
-    Parameter used_store_id : MemState -> store_id -> Prop.
 
     (*** Predicates *)
 
@@ -403,48 +193,29 @@ Module MemoryModelSpec (LP : LLVMParams) (MP : MemoryParams LP).
 
     (** Provenances / allocation ids *)
     Definition extend_allocation_ids (ms : MemState) (new_aid : AllocationId) (ms' : MemState) : Prop
-      := (forall aid, used_allocation_id ms aid -> used_allocation_id ms' aid) /\
-           ~ used_allocation_id ms new_aid /\
-           used_allocation_id ms' new_aid.
+      := (forall aid, used_allocation_id_prop ms aid -> used_allocation_id_prop ms' aid) /\
+           ~ used_allocation_id_prop ms new_aid /\
+           used_allocation_id_prop ms' new_aid.
 
     Definition preserve_allocation_ids (ms ms' : MemState) : Prop
-      := forall p, used_allocation_id ms p <-> used_allocation_id ms' p.
+      := forall p, used_allocation_id_prop ms p <-> used_allocation_id_prop ms' p.
 
     (** Store ids *)
     Definition extend_store_ids (ms : MemState) (new_sid : store_id) (ms' : MemState) : Prop
-      := (forall p, used_store_id ms p -> used_store_id ms' p) /\
-           ~ used_store_id ms new_sid /\
-           used_store_id ms' new_sid.
+      := (forall p, used_store_id_prop ms p -> used_store_id_prop ms' p) /\
+           ~ used_store_id_prop ms new_sid /\
+           used_store_id_prop ms' new_sid.
 
     Definition preserve_store_ids (ms ms' : MemState) : Prop
-      := forall sid, used_store_id ms sid <-> used_store_id ms' sid.
+      := forall sid, used_store_id_prop ms sid <-> used_store_id_prop ms' sid.
 
     (** Frame stack *)
     Definition frame_stack_preserved (m1 m2 : MemState) : Prop
       := forall fs,
-        mem_state_frame_stack m1 fs <-> mem_state_frame_stack m2 fs.
-
-    (*** Other helpers *)
-    Import MP.GEP.
-    Require Import List.
-    Import ListNotations.
-    Import LP.
-    Import ListUtil.
-    Import Utils.Monads.
-
-    (* TODO: Move this? *)
-    Definition intptr_seq (start : Z) (len : nat) : OOM (list IP.intptr)
-      := Util.map_monad (IP.from_Z) (Zseq start len).
-
-    Definition get_consecutive_ptrs (ptr : addr) (len : nat) : MemPropT (list addr) :=
-      ixs <- lift_OOM (intptr_seq 0 len);;
-      lift_err_RAISE_ERROR
-        (Util.map_monad
-           (fun ix => handle_gep_addr (DTYPE_I 8) ptr [DVALUE_IPTR ix])
-           ixs).
+        mem_state_frame_stack_prop m1 fs <-> mem_state_frame_stack_prop m2 fs.
 
     (*** Allocation id operations *)
-    Instance MemPropT_MonadAllocationId : MonadAllocationId AllocationId MemPropT.
+    Instance MemPropT_MonadAllocationId : MonadAllocationId AllocationId (MemPropT MemState).
     Proof.
       split.
       - (* fresh_allocation_id *)
@@ -463,7 +234,7 @@ Module MemoryModelSpec (LP : LLVMParams) (MP : MemoryParams LP).
     Defined.
 
     (*** Store id operations *)
-    Instance MemPropT_MonadStoreID : MonadStoreID MemPropT.
+    Instance MemPropT_MonadStoreID : MonadStoreID (MemPropT MemState).
     Proof.
       split.
       - (* fresh_sid *)
@@ -487,7 +258,7 @@ Module MemoryModelSpec (LP : LLVMParams) (MP : MemoryParams LP).
         read_byte_value : read_byte_prop ms ptr byte;
       }.
 
-    Definition read_byte_spec_MemPropT (ptr : addr) : MemPropT SByte:=
+    Definition read_byte_spec_MemPropT (ptr : addr) : MemPropT MemState SByte :=
       fun m1 res =>
            match res with
            | inr (NoOom (m2, byte)) => m1 = m2 /\ read_byte_spec m1 ptr byte
@@ -496,30 +267,30 @@ Module MemoryModelSpec (LP : LLVMParams) (MP : MemoryParams LP).
 
     (*** Framestack operations *)
     Definition empty_frame (f : Frame) : Prop :=
-      forall ptr, ~ ptr_in_frame f ptr.
+      forall ptr, ~ ptr_in_frame_prop f ptr.
 
     Record add_ptr_to_frame (f1 : Frame) (ptr : addr) (f2 : Frame) : Prop :=
       {
-        old_frame_lu : forall ptr', ptr_in_frame f1 ptr' -> ptr_in_frame f2 ptr';
-        new_frame_lu : ptr_in_frame f2 ptr;
+        old_frame_lu : forall ptr', ptr_in_frame_prop f1 ptr' -> ptr_in_frame_prop f2 ptr';
+        new_frame_lu : ptr_in_frame_prop f2 ptr;
       }.
 
     Record empty_frame_stack (fs : FrameStack) : Prop :=
       {
-        no_pop : (forall f, ~ pop_frame_stack fs f);
-        empty_fs_empty_frame : forall f, peek_frame_stack fs f -> empty_frame f;
+        no_pop : (forall f, ~ pop_frame_stack_prop fs f);
+        empty_fs_empty_frame : forall f, peek_frame_stack_prop fs f -> empty_frame f;
       }.
 
     Record push_frame_stack_spec (fs1 : FrameStack) (f : Frame) (fs2 : FrameStack) : Prop :=
       {
-        can_pop : pop_frame_stack fs2 fs1;
-        new_frame : peek_frame_stack fs2 f;
+        can_pop : pop_frame_stack_prop fs2 fs1;
+        new_frame : peek_frame_stack_prop fs2 f;
       }.
 
     Definition ptr_in_current_frame (ms : MemState) (ptr : addr) : Prop
-      := forall fs, mem_state_frame_stack ms fs ->
-               forall f, peek_frame_stack fs f ->
-                    ptr_in_frame f ptr.
+      := forall fs, mem_state_frame_stack_prop ms fs ->
+               forall f, peek_frame_stack_prop fs f ->
+                    ptr_in_frame_prop f ptr.
 
     (** mempush *)
     Record mempush_operation_invariants (m1 : MemState) (m2 : MemState) :=
@@ -535,16 +306,16 @@ Module MemoryModelSpec (LP : LLVMParams) (MP : MemoryParams LP).
       {
         fresh_frame :
         forall fs1 fs2 f,
-          mem_state_frame_stack m1 fs1 ->
+          mem_state_frame_stack_prop m1 fs1 ->
           empty_frame f ->
           push_frame_stack_spec fs1 f fs2 ->
-          mem_state_frame_stack m2 fs2;
+          mem_state_frame_stack_prop m2 fs2;
 
         mempush_invariants :
         mempush_operation_invariants m1 m2;
       }.
 
-    Definition mempush_spec_MemPropT : MemPropT unit :=
+    Definition mempush_spec_MemPropT : MemPropT MemState unit :=
       fun m1 res =>
         match res with
         | inr (NoOom (m2, _)) => mempush_spec m1 m2
@@ -581,15 +352,15 @@ Module MemoryModelSpec (LP : LLVMParams) (MP : MemoryParams LP).
         (* Set new framestack *)
         pop_frame :
         forall fs1 fs2,
-          mem_state_frame_stack m1 fs1 ->
-          pop_frame_stack fs1 fs2 ->
-          mem_state_frame_stack m2 fs2;
+          mem_state_frame_stack_prop m1 fs1 ->
+          pop_frame_stack_prop fs1 fs2 ->
+          mem_state_frame_stack_prop m2 fs2;
 
         (* Invariants *)
         mempop_invariants : mempop_operation_invariants m1 m2;
       }.
 
-    Definition mempop_spec_MemPropT : MemPropT unit :=
+    Definition mempop_spec_MemPropT : MemPropT MemState unit :=
       fun m1 res =>
         match res with
         | inr (NoOom (m2, _)) => mempop_spec m1 m2
@@ -599,9 +370,9 @@ Module MemoryModelSpec (LP : LLVMParams) (MP : MemoryParams LP).
     (* Add a pointer onto the current frame in the frame stack *)
     Definition add_ptr_to_frame_stack (fs1 : FrameStack) (ptr : addr) (fs2 : FrameStack) : Prop :=
       forall f f' fs1_pop,
-        peek_frame_stack fs1 f ->
+        peek_frame_stack_prop fs1 f ->
         add_ptr_to_frame f ptr f' ->
-        pop_frame_stack fs1 fs1_pop ->
+        pop_frame_stack_prop fs1 fs1_pop ->
         push_frame_stack_spec fs1_pop f' fs2.
 
     Fixpoint add_ptrs_to_frame_stack (fs1 : FrameStack) (ptrs : list addr) (fs2 : FrameStack) : Prop :=
@@ -640,7 +411,7 @@ Module MemoryModelSpec (LP : LLVMParams) (MP : MemoryParams LP).
         write_byte_invariants : write_byte_operation_invariants m1 m2;
       }.
 
-    Definition write_byte_spec_MemPropT (ptr : addr) (byte : SByte) : MemPropT unit
+    Definition write_byte_spec_MemPropT (ptr : addr) (byte : SByte) : MemPropT MemState unit
       := fun m1 res =>
            match res with
            | inr (NoOom (m2, _)) => write_byte_spec m1 ptr byte m2
@@ -658,12 +429,12 @@ Module MemoryModelSpec (LP : LLVMParams) (MP : MemoryParams LP).
         address_provenance : forall ptr, In ptr ptrs -> address_provenance ptr = allocation_id_to_prov aid;
 
         (* Allocation ids *)
-        allocate_bytes_aid_fresh : ~ used_allocation_id m1 aid;
-        allocate_bytes_aid : used_allocation_id m2 aid;
+        allocate_bytes_aid_fresh : ~ used_allocation_id_prop m1 aid;
+        allocate_bytes_aid : used_allocation_id_prop m2 aid;
         allocate_bytes_aids_preserved :
         forall aid',
           aid <> aid' ->
-          (used_allocation_id m1 aid' <-> used_allocation_id m2 aid');
+          (used_allocation_id_prop m1 aid' <-> used_allocation_id_prop m2 aid');
 
         (* byte_allocated *)
         allocate_bytes_was_fresh_byte : forall ptr, In ptr ptrs -> byte_not_allocated m1 ptr;
@@ -708,9 +479,9 @@ Module MemoryModelSpec (LP : LLVMParams) (MP : MemoryParams LP).
         (* Add allocated bytes onto the stack frame *)
         allocate_bytes_add_to_frame :
         forall fs1 fs2,
-          mem_state_frame_stack m1 fs1 ->
+          mem_state_frame_stack_prop m1 fs1 ->
           add_ptrs_to_frame_stack fs1 ptrs fs2 ->
-          mem_state_frame_stack m2 fs2;
+          mem_state_frame_stack_prop m2 fs2;
 
         (* Store ids are preserved. *)
         allocate_bytes_store_ids :
@@ -718,7 +489,7 @@ Module MemoryModelSpec (LP : LLVMParams) (MP : MemoryParams LP).
       }.
 
     Definition allocate_bytes_spec_MemPropT' (t : dtyp) (init_bytes : list SByte) (aid : AllocationId)
-      : MemPropT (addr * list addr)
+      : MemPropT MemState (addr * list addr)
       := fun m1 res =>
            match res with
            | inr (NoOom (m2, (ptr, ptrs))) =>
@@ -727,82 +498,311 @@ Module MemoryModelSpec (LP : LLVMParams) (MP : MemoryParams LP).
            end.
 
     Definition allocate_bytes_spec_MemPropT (t : dtyp) (init_bytes : list SByte)
-      : MemPropT addr
+      : MemPropT MemState addr
       := aid <- fresh_allocation_id;;
          '(ptr, _) <- allocate_bytes_spec_MemPropT' t init_bytes aid;;
          ret ptr.
 
+    (*** Initial memory state *)
+    Record initial_memory_state_prop : Prop :=
+      {
+        initial_memory_no_allocations :
+        forall ptr aid,
+          ~ byte_allocated initial_memory_state ptr aid;
+
+        initial_memory_frame_stack :
+        forall fs,
+          mem_state_frame_stack_prop initial_memory_state fs ->
+          empty_frame_stack fs;
+
+        initial_memory_no_reads :
+        forall ptr byte,
+          ~ read_byte_prop initial_memory_state ptr byte
+      }.
+
+    Record initial_frame_prop : Prop :=
+      {
+        initial_frame_is_empty : empty_frame initial_frame;
+      }.
+
     (*** Aggregate things *)
 
     (** Reading uvalues *)
-    Definition read_bytes_spec (ptr : addr) (len : nat) : MemPropT (list SByte) :=
+    Definition read_bytes_spec (ptr : addr) (len : nat) : MemPropT MemState (list SByte) :=
+      (* TODO: should this OOM, or should this count as walking outside of memory and be UB? *)
       ptrs <- get_consecutive_ptrs ptr len;;
 
       (* Actually perform reads *)
       Util.map_monad (fun ptr => read_byte_spec_MemPropT ptr) ptrs.
 
-    Definition read_uvalue_spec (dt : dtyp) (ptr : addr) : MemPropT uvalue :=
+    Definition read_uvalue_spec (dt : dtyp) (ptr : addr) : MemPropT MemState uvalue :=
       bytes <- read_bytes_spec ptr (N.to_nat (sizeof_dtyp dt));;
       ret (from_ubytes bytes dt).
 
     (** Writing uvalues *)
-    Definition write_bytes_spec (ptr : addr) (bytes : list SByte) : MemPropT unit :=
+    Definition write_bytes_spec (ptr : addr) (bytes : list SByte) : MemPropT MemState unit :=
       ptrs <- get_consecutive_ptrs ptr (length bytes);;
       let ptr_bytes := zip ptrs bytes in
 
       (* Actually perform writes *)
       Util.map_monad_ (fun '(ptr, byte) => write_byte_spec_MemPropT ptr byte) ptr_bytes.
 
-    Definition write_uvalue_spec (dt : dtyp) (ptr : addr) (uv : uvalue) : MemPropT unit :=
+    Definition write_uvalue_spec (dt : dtyp) (ptr : addr) (uv : uvalue) : MemPropT MemState unit :=
       sid <- fresh_sid;;
       bytes <- lift_OOM (to_ubytes uv dt sid);;
       write_bytes_spec ptr bytes.
 
     (** Allocating dtyps *)
-    Definition generate_undef_bytes (dt : dtyp) (sid : store_id) : OOM (list SByte) :=
-      N.recursion
-        (fun (x : N) => ret [])
-        (fun n mf x =>
-           rest_bytes <- mf (N.succ x);;
-           x' <- IP.from_Z (Z.of_N x);;
-           let byte := uvalue_sbyte (UVALUE_Undef dt) dt (UVALUE_IPTR x') sid in
-           ret (byte :: rest_bytes))
-        (sizeof_dtyp dt) 0%N.
-
     (* Need to make sure MemPropT has provenance and sids to generate the bytes. *)
-    Definition allocate_dtyp_spec (dt : dtyp) : MemPropT addr :=
+    Definition allocate_dtyp_spec (dt : dtyp) : MemPropT MemState addr :=
       sid <- fresh_sid;;
       bytes <- lift_OOM (generate_undef_bytes dt sid);;
       allocate_bytes_spec_MemPropT dt bytes.
 
     (*** Handling memory events *)
-    Definition handle_memory_prop : MemoryE ~> MemPropT
+    Section Handlers.
+      Definition handle_memory_prop : MemoryE ~> MemPropT MemState
+        := fun T m =>
+             match m with
+             (* Unimplemented *)
+             | MemPush =>
+                 mempush_spec_MemPropT
+             | MemPop =>
+                 mempop_spec_MemPropT
+             | Alloca t =>
+                 addr <- allocate_dtyp_spec t;;
+                 ret (DVALUE_Addr addr)
+             | Load t a =>
+                 match a with
+                 | DVALUE_Addr a =>
+                     read_uvalue_spec t a
+                 | _ =>
+                     (* UB if loading from something that isn't an address *)
+                     fun _ _ => False
+                 end
+             | Store t a v =>
+                 match a with
+                 | DVALUE_Addr a =>
+                     write_uvalue_spec t a v
+                 | _ =>
+                     (* UB if writing something to somewhere that isn't an address *)
+                     fun _ _ => False
+                 end
+             end.
+    End Handlers.
+End MemoryModelSpec.
+
+Module MakeMemoryModelSpec (LP : LLVMParams) (MP : MemoryParams LP) (MMSP : MemoryModelSpecPrimitives LP MP) <: MemoryModelSpec LP MP MMSP.
+  Include MemoryModelSpec LP MP MMSP.
+End MakeMemoryModelSpec.
+
+Module Type MemoryModelExecPrimitives (LP : LLVMParams) (MP : MemoryParams LP) (MMSP : MemoryModelSpecPrimitives LP MP).
+  Import LP.
+  Import LP.ADDR.
+  Import LP.SIZEOF.
+  Import LP.PROV.
+  Import MP.
+  Import MMSP.
+  Import MMSP.MemByte.
+
+  Module MemSpec := MakeMemoryModelSpec LP MP MMSP.
+  Import MemSpec.
+
+  Section MemoryPrimatives.
+    Context {MemM : Type -> Type}.
+    Context `{MemMonad MemState AllocationId MemM}.
+
+    (*** Primitives on memory *)
+    (** Reads *)
+    Parameter read_byte : addr -> MemM SByte.
+
+    (** Writes *)
+    Parameter write_byte : addr -> SByte -> MemM unit.
+
+    (** Allocations *)
+    Parameter addr_allocated : addr -> AllocationId -> MemM bool. (* TODO: do we need this? *)
+    Parameter allocate_bytes : dtyp -> list SByte -> MemM addr.
+
+    (** Frame stacks *)
+    (* Check if an address is allocated in a frame *)
+    Parameter ptr_in_frame : Frame -> addr -> bool.
+
+    (* Check for the current frame *)
+    Parameter peek_frame_stack : FrameStack -> Frame.
+    Parameter push_frame_stack : FrameStack -> Frame -> FrameStack.
+    Parameter pop_frame_stack : FrameStack -> err FrameStack.
+
+    Parameter mem_state_frame_stack : MemState -> FrameStack.
+    Parameter mem_state_set_frame_stack : MemState -> FrameStack -> MemState.
+
+    (** Allocation ids / store ids *)
+    Parameter used_allocation_id : MemState -> AllocationId -> bool.
+    Parameter used_store_id : MemState -> store_id -> bool.
+
+    (*** Correctness *)
+    Import EitherMonad.
+    Definition exec_correct {X} (exec : MemM X) (spec : MemPropT MemState X) : Prop :=
+      forall ms,
+        match IdentityMonad.unIdent (unEitherT (unEitherT (unEitherT (unERR_UB_OOM (MemMonad_runs_to exec ms))))) with
+        | inl (OOM_message oom_msg) =>
+            spec ms (inr (Oom oom_msg))
+        | inr (inl (UB_message ub_msg)) =>
+            forall res, ~ spec ms res
+        | inr (inr (inl (ERR_message err_msg))) =>
+            spec ms (inl err_msg)
+        | inr (inr (inr (ms', res))) =>
+            spec ms (inr (NoOom (ms', res)))
+        end.
+
+    (** Correctness of the main operations on memory *)
+    Parameter read_byte_correct :
+      forall ptr, exec_correct (read_byte ptr) (read_byte_MemPropT ptr).
+
+    Parameter write_byte_correct :
+      forall ptr byte, exec_correct (write_byte ptr byte) (write_byte_spec_MemPropT ptr byte).
+
+    (* TODO: do I need this at all? *)
+    Parameter addr_allocated_correct :
+      forall ptr aid, exec_correct (addr_allocated ptr aid) (addr_allocated_prop ptr aid).
+
+    Parameter allocate_bytes_correct :
+      forall dt init_bytes, exec_correct (allocate_bytes dt init_bytes) (allocate_bytes_spec_MemPropT dt init_bytes).
+
+    (** Correctness of frame stack operations *)
+    Parameter ptr_in_frame_correct :
+      forall frame ptr,
+        ptr_in_frame_prop frame ptr <->
+        ptr_in_frame frame ptr = true.
+
+    Parameter peek_frame_stack_correct :
+      forall frame_stack frame,
+        peek_frame_stack_prop frame_stack frame <->
+          peek_frame_stack frame_stack = frame.
+
+    Parameter push_frame_stack_correct :
+      forall frame_stack frame_stack' frame,
+        push_frame_stack_spec frame_stack frame frame_stack' <->
+          push_frame_stack frame_stack frame = frame_stack'.
+
+    Parameter pop_frame_stack_correct :
+      forall frame_stack frame,
+        pop_frame_stack_prop frame_stack frame <->
+          pop_frame_stack frame_stack = inr frame.
+
+    Parameter mem_state_frame_stack_correct :
+      forall ms fs,
+        mem_state_frame_stack_prop ms fs <->
+          mem_state_frame_stack ms = fs.
+
+    Record mem_state_set_frame_stack_invariants (m1 : MemState) (m2 : MemState) :=
+      {
+        mem_state_set_frame_stack_op_reads : read_byte_preserved m1 m2;
+        mem_state_set_frame_stack_op_write_allowed : write_byte_allowed_all_preserved m1 m2;
+        mem_state_set_frame_stack_op_allocations : allocations_preserved m1 m2;
+        mem_state_set_frame_stack_op_store_ids : preserve_store_ids m1 m2;
+        mem_state_set_frame_stack_op_allocation_ids : preserve_allocation_ids m1 m2;
+      }.
+
+    Parameter mem_state_set_frame_stack_correct :
+      forall ms ms' fs,
+        (mem_state_frame_stack_prop ms' fs /\ mem_state_set_frame_stack_invariants ms ms') <->
+          mem_state_set_frame_stack ms fs = ms'.
+
+    (** Allocation ids / store ids *)
+    Parameter used_allocation_id_correct :
+      forall ms aid,
+        used_allocation_id_prop ms aid <-> used_allocation_id ms aid = true.
+
+    Parameter used_store_id_correct :
+      forall ms aid,
+        used_store_id_prop ms aid <-> used_store_id ms aid = true.
+  End MemoryPrimatives.
+End MemoryModelExecPrimitives.
+
+Module Type MemoryModelExec (LP : LLVMParams) (MP : MemoryParams LP) (MMSP : MemoryModelSpecPrimitives LP MP) (MMEP : MemoryModelExecPrimitives LP MP MMSP).
+  Import LP.
+  Import LP.ADDR.
+  Import LP.SIZEOF.
+  Import LP.PROV.
+  Import LP.Events.
+  Import MP.
+  Import MMSP.
+  Import MMSP.MemByte.
+  Import MMEP.
+  Import MMEP.MemSpec.
+  Import MemHelpers.
+
+  (*** Handling memory events *)
+  Section Handlers.
+    Variable MemM : Type -> Type.
+    Context `{MemMonad MemState AllocationId MemM}.
+
+    (** Reading uvalues *)
+    Definition read_bytes (ptr : addr) (len : nat) : MemM (list SByte) :=
+      (* TODO: this should maybe be UB and not OOM??? *)
+      ptrs <- get_consecutive_ptrs ptr len;;
+
+      (* Actually perform reads *)
+      Util.map_monad (fun ptr => read_byte ptr) ptrs.
+
+    Definition read_uvalue (dt : dtyp) (ptr : addr) : MemM uvalue :=
+      bytes <- read_bytes ptr (N.to_nat (sizeof_dtyp dt));;
+      ret (from_ubytes bytes dt).
+
+    (** Writing uvalues *)
+    Definition write_bytes (ptr : addr) (bytes : list SByte) : MemM unit :=
+      (* TODO: Should this be UB instead of OOM? *)
+      ptrs <- get_consecutive_ptrs ptr (length bytes);;
+      let ptr_bytes := zip ptrs bytes in
+
+      (* Actually perform writes *)
+      Util.map_monad_ (fun '(ptr, byte) => write_byte ptr byte) ptr_bytes.
+
+    Definition write_uvalue (dt : dtyp) (ptr : addr) (uv : uvalue) : MemM unit :=
+      sid <- fresh_sid;;
+      bytes <- lift_OOM (to_ubytes uv dt sid);;
+      write_bytes ptr bytes.
+
+    (** Allocating dtyps *)
+    (* Need to make sure MemPropT has provenance and sids to generate the bytes. *)
+    Definition allocate_dtyp (dt : dtyp) : MemM addr :=
+      sid <- fresh_sid;;
+      bytes <- lift_OOM (generate_undef_bytes dt sid);;
+      allocate_bytes dt bytes.
+
+    Definition handle_memory_prop : MemoryE ~> MemM
       := fun T m =>
            match m with
            (* Unimplemented *)
            | MemPush =>
-               mempush_spec_MemPropT
+               ms <- get_mem_state;;
+               let fs := mem_state_frame_stack ms in
+               let fs' := push_frame_stack fs initial_frame in
+               let ms' := mem_state_set_frame_stack ms fs' in
+               put_mem_state ms'
            | MemPop =>
-               mempop_spec_MemPropT
+               ms <- get_mem_state;;
+               let fs := mem_state_frame_stack ms in
+               fs' <- lift_err_RAISE_ERROR (pop_frame_stack fs);;
+               let ms' := mem_state_set_frame_stack ms fs' in
+               put_mem_state ms'
            | Alloca t =>
-               addr <- allocate_dtyp_spec t;;
+               addr <- allocate_dtyp t;;
                ret (DVALUE_Addr addr)
            | Load t a =>
                match a with
                | DVALUE_Addr a =>
-                   read_uvalue_spec t a
+                   read_uvalue t a
                | _ =>
-                   (* UB if loading from something that isn't an address *)
-                   fun _ _ => False
+                   raise_ub "Loading from something that is not an address."
                end
            | Store t a v =>
                match a with
                | DVALUE_Addr a =>
-                   write_uvalue_spec t a v
+                   write_uvalue t a v
                | _ =>
-                   (* UB if writing something to somewhere that isn't an address *)
-                   fun _ _ => False
+                   raise_ub "Store to somewhere that is not an address."
                end
            end.
   End Handlers.
-End MemoryModelSpec.
+End MemoryModelExec.
