src/coq/Handlers/MemPropT.v
@@ -1,0 +1,170 @@
+From Coq Require Import ZArith.
+
+From ExtLib Require Import
+     Structures.Monad.
+
+From ITree Require Import
+     ITree
+     Basics.Basics
+     Events.StateFacts
+     Events.State.
+
+From Vellvm Require Import Error.
+
+From Vellvm.Semantics Require Import
+     MemoryAddress
+     LLVMEvents.
+
+Import Basics.Basics.Monads.
+Import MonadNotation.
+Open Scope monad_scope.
+
+(* Move this ? *)
+Definition store_id := N.
+Class MonadStoreID (M : Type -> Type) : Type :=
+  { fresh_sid : M store_id;
+  }.
+
+Class MonadMemState (MemState : Type) (M : Type -> Type) : Type :=
+  { get_mem_state : M MemState;
+    put_mem_state : MemState -> M unit;
+  }.
+
+Definition modify_mem_state {M MemState} `{Monad M} `{MonadMemState MemState M} (f : MemState -> MemState) : M MemState :=
+  ms <- get_mem_state;;
+  put_mem_state (f ms);;
+  ret ms.
+
+(* TODO: Add RAISE_PICK or something... May need to be in a module *)
+Class MemMonad (MemState : Type) (AllocationId : Type) (M : Type -> Type)
+      `{Monad M}
+      `{MonadAllocationId AllocationId M} `{MonadStoreID M} `{MonadMemState MemState M}
+      `{RAISE_ERROR M} `{RAISE_UB M} `{RAISE_OOM M} : Type
+  :=
+  {
+    MemMonad_runs_to {A} (ma : M A) (ms : MemState) : err_ub_oom (MemState * A);
+    MemMonad_lift_stateT
+      {E} `{FailureE -< E} `{UBE -< E} `{OOME -< E} {A}
+      (ma : M A) : stateT MemState (itree E) A;
+  }.
+
+
+Definition MemPropT (MemState : Type) (X : Type) : Type
+  := MemState -> err (OOM (MemState * X)%type) -> Prop.
+
+(* Instance MemPropT_Monad : Monad MemPropT. *)
+(* Proof. *)
+(*   split. *)
+(*   - (* ret *) *)
+(*     intros T x. *)
+(*     unfold MemPropT. *)
+(*     intros ms [err_msg | [[ms' res] | oom_msg]]. *)
+(*     + exact False. (* error is not a valid behavior here *) *)
+(*     + exact (ms = ms' /\ x = res). *)
+(*     + exact True. (* Allow OOM to refine anything *) *)
+(*   - (* bind *) *)
+(*     intros A B ma amb. *)
+(*     unfold MemPropT in *. *)
+
+(*     intros ms [err_msg | [[ms'' b] | oom_msg]]. *)
+(*     + (* an error is valid when ma errors, or the continuation errors... *) *)
+(*       refine *)
+(*         ((exists err, ma ms (inl err)) \/ *)
+(*          (exists ms' a, *)
+(*              ma ms (inr (NoOom (ms', a))) -> *)
+(*              (exists err, amb a ms' (inl err)))). *)
+(*     + (* No errors, no OOM *) *)
+(*       refine *)
+(*         (exists ms' a k, *)
+(*             ma ms (inr (NoOom (ms', a))) -> *)
+(*             amb a ms' (inr (NoOom (ms'', k a)))). *)
+(*     + (* OOM is always valid *) *)
+(*       exact True. *)
+(* Defined. *)
+
+(* To triple check, but the following makes more sense to me *)
+Instance MemPropT_Monad {MemState : Type} : Monad (MemPropT MemState).
+Proof.
+  split.
+  - (* ret *)
+    refine (fun _ v s r => match r with
+                        | inl _ => False
+                        | inr (NoOom (s',r')) => s' = s /\ r' = v
+                        | inr (Oom _) => True
+                        end).
+  - (* bind *)
+    refine (fun A B ma amb sa r =>
+              match r with
+              | inl err            =>
+                  ma sa (inl err) \/
+                    (exists sab a, ma sa (inr (NoOom (sab, a))) /\
+                                (exists err, amb a sab (inl err)))
+              | inr (NoOom (sb,r)) =>
+                  exists sab a,
+                  ma    sa  (inr (NoOom (sab, a))) /\
+                    amb a sab (inr (NoOom (sb, r)))
+              | inr (Oom _)         => True
+              end
+           ).
+Defined.
+
+Instance MemPropT_MonadMemState {MemState : Type} : MonadMemState MemState (MemPropT MemState).
+Proof.
+  split.
+  - (* get_mem_state *)
+    unfold MemPropT.
+    intros ms [err_msg | [[ms' a] | oom_msg]].
+    + exact True.
+    + exact (ms = ms' /\ a = ms).
+    + exact True.
+  - (* put_mem_state *)
+    unfold MemPropT.
+    intros ms_to_put ms [err_msg | [[ms' t] | oom_msg]].
+    + exact True.
+    + exact (ms_to_put = ms').
+    + exact True.
+Defined.
+
+Instance MemPropT_RAISE_OOM {MemState : Type} : RAISE_OOM (MemPropT MemState).
+Proof.
+  split.
+  - intros A msg.
+    unfold MemPropT.
+    intros ms [err | [_ | oom]].
+    + exact False. (* Must run out of memory, can't error *)
+    + exact False. (* Must run out of memory *)
+    + exact True. (* Don't care about message *)
+Defined.
+
+Instance MemPropT_RAISE_ERROR {MemState : Type} : RAISE_ERROR (MemPropT MemState).
+Proof.
+  split.
+  - intros A msg.
+    unfold MemPropT.
+    intros ms [err | [_ | oom]].
+    + exact True. (* Any error will do *)
+    + exact False. (* Must error *)
+    + exact False. (* Must error *)
+Defined.
+
+Definition MemPropT_assert {MemState X} (assertion : Prop) : MemPropT MemState X
+  := fun ms ms'x =>
+       match ms'x with
+       | inl _ =>
+           assertion
+       | inr (NoOom (ms', x)) =>
+           ms = ms' /\ assertion
+       | inr (Oom s) =>
+           assertion
+       end.
+
+Definition MemPropT_assert_post {MemState X} (Post : X -> Prop) : MemPropT MemState X
+  := fun ms ms'x =>
+       match ms'x with
+       | inl _ =>
+           True
+       | inr (NoOom (ms', x)) =>
+           ms = ms' /\ Post x
+       | inr (Oom s) =>
+           True
+       end.
